---
published: true
title: 'Chapter 1.2 [Excursions] II'
layout: post
date: '2021-08-20 15:56:07 +0700'
categories: misc
permalink: '/:categories/2'
---
{% include katex.html %}

## Metric Preserving Functions

For any metric space \\( (M,d) \\), a function \\( f:[0,\infty) \to [0,\infty) \\) is said to be metric preserving if \\( f\circ d \\) is a metric on \\( M \\). Sometimes we will write \\( d_f \\) instead of \\( f\circ d \\) for simplicity.

> Unless otherwise specified, anytime a function is mentioned it is to be understood that it has domain \\( [0,\infty) \\) and codomain \\( [0,\infty) \\). 

There is an easy way to determine whether or not a function is metric preserving, we simply need to check if the following properties are satisfied:

- \\( f(x)=0 \\) if and only if \\( x=0 \\).
- \\( f \\) is increasing.
- \\( f \\) is subadditive.

> For those unfamiliar with subadditivity, a function is said to be subadditive if 
\\[ f(x+y)\leq f(x)+f(y), \\]
for all \\( x,y \\) in the domain of \\( f \\).

It is easy to see that the first condition in the list ensures that the first property of the metric is satisfied, the other two conditions on the list ensures that the triangle inequality hold. The second property of the metric is automatically/immediately satisfied. We shall only prove that the last the conditions imply the triangle inequality. 

Proof. Let \\( (M,d) \\) be a metric space. For any \\( x,y,z\in M \\), we have \\( d(x,z)\leq d(x,y)+d(y,z) \\), and since \\( f \\) is increasing and subadditive,

\\[ d_f(x,z)\leq f(d(x,y)+d(y,z))\leq d_f(x,y)+d_f(y,z). \\]

Thus, \\( d_f \\) satisfies the triangle inequality. \\( \Box \\)



> Definition. We say that a real-valued function defined on an interval, \\( I \\), is concave if given any \\( t\in [0,1] \\), we have
\\[ \text{for all }x,y\in I, \quad f(tx+(1-t)y)\geq tf(x)+(1-t)f(y). \tag{1} \\]

An example of a concave function is \\( f(x)=\sqrt{x} \\),

Proof. We need to show that for any \\( t\in [0,1] \\) and \\( x,y\in [0,\infty) \\), 

\\[ \sqrt{tx+(1-t)y}\geq t\sqrt{x}+(1-t)\sqrt{y}. \\]

By AM-GM, we have \\( \frac{x+y}{2}\geq \sqrt{xy} \\), multiplying by \\( 2t(1-t) \\) gives

\\[ t(1-t)(x+y)\geq 2t(1-t)\sqrt{x}\sqrt{y}. \\]

Note: \\( 2t(1-t)\geq 0 \\) because \\( t\in [0,1] \\). We will now add \\( t^2x+(1-t)^2y \\) on both sides, after simplification, this results in

\\[ tx+(1-t)y\geq t^2x+2t(1-t)\sqrt{x}\sqrt{y}+(1-t)^2y. \\]

Taking the square root on both sides gives the desired inequality. \\( \Box \\)

> Claim. Suppose that \\( f \\) is a concave function defined on the interval \\( [0,\infty) \\), that \\( f(x)=0 \\) iff \\( x=0 \\), and that \\( f \\) is increasing, then if \\( M \\) is a metric space with a metric \\( d \\), the composition \\( f\circ d \\) is also a metric on \\( M \\).

Proof. We prove the triangle inequality only, since \\( d \\) is a metric, for any three points \\( x,y,z\in M \\), we have

\\[ d(x,z)\leq d(x,y)+d(y,z), \\]

therefore,

\\[ f(d(x,z))\leq f(d(x,y)+d(y,z)) \\]

If we manage can manage to prove that \\( f(x+y)\leq f(x)+f(y) \\) for any \\( x,y\geq 0 \\), then we are done.

- By letting \\( y=0 \\) in (1) we obtain \\( f(tx)\geq tf(x) \\) for any \\( x\in [0,\infty) \\) and \\( t\in [0,1] \\).

Let \\( x,y \\) be arbitrary points in \\( [0,\infty) \\), then we can set \\( t=\frac{x}{x+y}\in[0,1] \\),

\\[ \begin{align\*} f(x)&=f(t(x+y))\geq tf(x+y) \newline f(y)&=f((1-t)(x+y))\geq (1-t)f(x+y)\end{align\*} \\]

Therefore, 

\\[ f(x)+f(y)\geq tf(x+y)+(1-t)f(x+y)=f(x+y). \quad \Box \\]
