---
published: true
layout: post
categories: Set-Theory
permalink: '/:categories/8'
---
{% include katex.html %}

We wish to answer the following question: Suppose we are given a set \\( A \\), an element \\( a\in A \\), and a function \\( F:A\to A \\). Can we find a function \\( h:\omega\to A \\) such that (1) \\( h(0)=a \\) and (2) \\( h(n^+)=F(h(n)) \\) for all \\( n\in \omega \\)? If the function exists, it must obey

\\[ h(0)=a, \quad h(1)=F(h(0))=F(a), \quad h(2)=F(h(1))=F(F(a)). \\]

i.e,

\\[ h=\\{<n,F^n(a)> \ \vert \ n\in \omega\\} \\]

where \\( F^n=\overbrace{F(F(\cdots}^{n\text{ times}}(a))) \\) with \\( F^0=a \\). With \\( h \\) defined this way, clearly \\( h(0)=a \\) and \\( h(n^+)=F(F^n(n))=F(h(n)) \\), so the requirements are satisfied. The problem with this proposal is that it is not entirely clear if we can explicitly construct the set \\( h \\). If we could, that would mean that we can encode the idea of recursion within set theory. This is possible to do, but to show why is not an easy task.

> Theorem 2.2.1 [Recursion Theorem] Let \\( A \\) be a set, \\( a\in A \\), and \\( F:A\to A \\). Then there exists a unique function \\( h:\omega\to A \\) such that \\( h(0)=a \\) and \\( h(n^+)=F(h(n)) \\) for all \\( n\in \omega \\).

Proof. First we prove uniqueness. Suppose there is some other function \\( g \\) with the same properties as \\( h \\). Let \\( V=\\{ n\in \omega \ \vert \ g(n)=h(n) \\} \\), then if we can prove that \\( V=\omega \\) this would clearly show \\( g=h \\). We will do this via induction. We know that \\( 0\in V \\) because \\( h(0)=g(0)=a \\). Now assume that we have some \\( n\in V \\), this means \\( g(n)=h(n) \\). Then 

\\[ h(n^+)=F(h(n))=F(g(n))=g(n^+) \\]

so \\( n^+\in V \\) as needed. Now we shall prove existence. Define

\\[ \mathcal{K}=\\{ v\subseteq \omega \times A \ \vert \ <0,a>\in v, \ (\forall n,y) \ <n,y>\in v \ \rightarrow \ <n^+, F(y)>\in v \\} \\]

Then we shall show that \\( h=\bigcap \mathcal{K} \\) has the desired properties. First note that \\( \mathcal{K} \\) is nonempty because clearly \\( \omega\times A\in \mathcal{K} \\). It is also clear that \\( h\subseteq \omega \times A \\). Now we will show that \\( h\in \mathcal{K} \\), this will be done in the next paragraph

Every \\( v\in \mathcal{K} \\) contains \\( <0,a> \\), so it is clear that \\( <0,a>\in h \\). Next, suppose that \\( <n,y>\in h \\). Choose any \\( v\in \mathcal{K} \\), then we know that \\( <n,y>\in v \ \rightarrow \ <n^+,F(y)>\in v \\). This means that \\( \forall v\in \mathcal{K}, \ <n^+,y>\in v \\), i.e, \\( <n^+,F(y)>\in h \\) as needed. This shows that \\( h\in \mathcal{K} \\).

Before continuing, we shall prove a Lemma: if we are provided with an \\( <n,y>\in h \\) (with \\( <n,y>\neq <0,a> \\)), then we can find some \\( <m,u>\in h \\) such that \\( <m^+,F(u)>=<n,y> \\).

Proof. Suppose on the contrary that there is some \\( <r,t>\in h \\) (with \\( <r,t>\neq <0,a> \\)) for which there is no ordered pair \\( <m,u>\in h \\) satisfying \\( <r,t>=<m^+,F(u)> \\). We shall create a new set \\( \hat{h}=h-\\{<r,t>\\} \\). Clearly \\( \hat{h}\subseteq \omega\times A \\). We now wish to show that \\( \hat{h}\in \mathcal{K} \\).

First, note that \\( <0,a>\in \hat{h} \\) because only \\( <r,t> \\) was removed to create \\( \hat{h} \\) and \\( <r,t>\neq <0,a> \\). Now suppose \\( <n,y>\in \hat{h} \\), then by construction \\( <n,y>\in h \ \rightarrow \ <n^+,F(y)>\in h \\) <- since \\( h\in \mathcal{K} \\). By assumption we know that \\( <n^+,F(y)>\neq <r,t> \\), so \\( <n^+,F(y)>\in \hat{h} \\). This shows that \\( \hat{h}\in \mathcal{K} \\), but this is impossible since that would imply \\( h\subseteq \hat{h} \\). (remember \\( \bigcap \mathcal{K}=h\subseteq v \\) for all \\( v\in \mathcal{K} \\))

We continue by proving that \\( h:\omega \to A \\) is a function. To do this we define

\\[ G=\\{ n\in \omega \ \vert \ \exists! x \ <n,x>\in h \\} \\]

If we can show that \\( G=\omega \\) (via induction), this will show that \\( h \\) is a function with domain \\( \omega \\). That \\( h \\) has codomain \\( A \\) should be obvious. Because \\( h\in \mathcal{K} \\) we know that \\( <0,a>\in h \\) but this is not enough, we need to show that \\( 0 \\) is not mapped to any other element. Suppose that there exist a \\( p\in A \\) (\\( p\neq a \\)) such that \\( <0,p>\in h \\). By the lemma, we can find some \\( <m,u>\in h \\) such that \\( <m^+,F(u)>=<0,p> \\), but this implies that \\( m^+=0 \\). Recall that \\( <\omega, \sigma, 0> \\) form a Peano system. \\( m^+=\sigma(m)=0 \\) is a contradiction because \\( 0\notin \text{ran }\sigma \\) is one of the postulates of a Peano system. Hence, \\( 0\in G \\).

Now suppose \\( n\in G \\). Then there is a unique \\( y\in A \\) such that \\( <n,y>\in h \\). Because \\( h\in \mathcal{K} \\) we have that \\( <n^+,F(y)>\in h \\). We now need to show that \\( F(y) \\) is the only thing that \\( n^+ \\) maps to. We prove by contradiction, suppose that there is some other \\( q\in A \\) such that \\( <n^+,q>\in h \\). We know that \\( n^+\neq 0 \\) by the postulates, and hence \\( <n^+,q>\neq <0,a> \\) so we can apply the lemma. We can then find \\( <a,b>\in h \\) such that \\( <a^+,F(b)>=<n^+,q> \\). We know that \\( a=n \\) this is because the successor function is injective per the postulates. Thus \\( <a,b>=<n,b>\in h \\). Since \\( n \\) is mapped uniquely to \\( y \\) we must have \\( b=y \\). Hence \\( q=F(b)=F(y) \\). This is a contradiction because we assumed that \\( q \\) was distinct from \\( F(y) \\). Thus, \\( n^+\in G \\) as needed. By induction we have shown \\( G=\omega \\).

Finally we show that \\( h(0)=a \\) and \\( h(n^+)=F(h(n)) \\) for all \\( n\in \omega \\). \\( h(0)=a \\) is equivalent to \\( <0,a>\in h \\) which we have already shown. Assume \\( n\in \omega \\), then \\( <n,h(n)>\in h \\) <- we have shown that \\( h \\) is a function so all is good here. Since \\( h\in \mathcal{K} \\) we have \\( <n^+,F(h(n))>\in h \\), i.e, \\( h(n^+)=F(h(n)) \\) as needed. \\( \Box \\)

By uniqueness we know that

\\[ \bigcap \mathcal{K}=\\{ <n,F^n(a)> \ \vert \ n\in \omega \\} \\]

i.e, the function we proposed early on in this post is something that can be constructed from the base axioms. As an application of the recursion theorem, we shall prove the following:

> Theorem 2.2.2 Let \\( <N,S,e> \\) be a Peano system. Then \\( <\omega, \sigma, 0> \\) is isomorphic to \\( <N,S,e> \\) in the sense that there exists a function \\( h:\omega \to N \\) that is one-to-one and
\\[ h(0)=e, \quad \text{and} \quad h(\sigma(n))=S(h(n)), \text{ for all }n\in \omega. \\]

The diagram below shows what \\( h \\) should look like should it exist

![Capture.PNG](/MathBlog/assets/Capture20.PNG)

It looks like we need recursion to define a function \\( h \\) so that

\\[ h(0)=e, \quad h(1)=S(e), \quad h(2)=S(S(e)), \quad \cdots \\]

In short, we would say \\( h \\) is defined by recursion of the function \\( S \\) with the seed \\( e \\). Before we attempt this idea, it turns out that we need the following lemma:

> Lemma 2.2.3 Let \\( f:A\to A \\) be one-to-one, and assume that \\( c\in A-\text{ran} f \\). Define \\( h \\) by recursion of \\( f \\) with seed \\( c \\). Then \\( h \\) is one-to-one. 
