---
published: true
---
{% include katex.html %}

We have already defined numbers but not yet operations such as addition, multiplication, etc.. Recursion is needed for this task, that is why it was important to understand that topic hard as it may be. How should we think of addition in terms of set theory? For example let us say we want to take a number \\( n\in \omega \\) and add it by \\( 3 \\). We can do this by applying the successor operation three times on \\( n \\), i.e, the addition of \\( n \\) and \\( 3 \\) gives:

\\[ \sigma(\sigma(\sigma(n)))=n^{+++} \\] 

Obviously recursion should be involved somehow. If we define a function \\( A_n \\) by recursion of \\( \sigma \\) with seed \\( n \\), then \\( A_n(3)=\sigma^3(n) \\). In general, for any two \\( n,m\in \omega \\) we can define \\( n+m \\) to be equivalent to \\( A_n(m)=\sigma^m(n) \\).

> Theorem 2.3.1 For any \\( n,m\in \omega \\) we have
- \\( n+0=n \\)
- \\( n+m^+=(n+m)^+ \\)

Proof. Remember that \\( A_n \\) has seed \\( n \\) so \\( n+0=A_n(0)=n \\). Next,

\\[ n+m^+=A_n(m^+)=\sigma(A_n(m))=\sigma(n+m). \quad \Box \\]

We now move on to multiplication. We define a function \\( M_n \\) by recursion of \\( A_n \\) with seed \\( 0 \\). For example, 

\\[ M_2(3)=A_2(A_2(A_2(0)))=(2+(2+(2+0))) \\]

which, after a lot of steps, evaluates to \\( 6 \\). In general for any \\( n,m\in \omega \\) we define the multiplication, \\( n\cdot m \\) to be equivalent to \\( M_n(m) \\).

> Theorem 2.3.2 For any \\( n,m\in \omega \\) we have
- \\( n\cdot 0=0 \\)
- \\( n\cdot 1=n \\)
- \\( n\cdot m^+=n+n\cdot m \\)

Proof. First, \\( n\cdot 0=M_n(0)=0 \\) since \\( M_n \\) has seed \\( 0 \\). Next, \\( n\cdot 1=M_n(1)=A_n(0)=n \\). Finally,

\\[ n\cdot m^+=M_n(m^+)=A_n(M_n(m))=n+M_n(m)=n+n\cdot m. \quad \Box \\]

We can also define exponentiation. Define a function \\( E_n \\) be recursion of \\( M_n \\) with seed \\( 1 \\). For any \\( n,m\in \omega \\) we define the exponentiation, \\( n^m \\), to be equivalent to \\( E_n(m) \\). 

> Theorem 2.3.3 for any \\( n,m,p\in \omega \\),
- Associative law for addition
\\[ n+(m+p)=(n+m)+p \\]
- Commutative law for addition
\\[ n+m=m+n \\]
- Distributive law
\\[ n\cdot (m+p)=n\cdot m + n\cdot p \\]
- Associative law for multiplication
\\[ n\cdot (m\cdot p)=(n\cdot m)\cdot p \\]
- Commutative law for multiplication
\\[ n\cdot m=m\cdot n \\]

The proof is tedious, boring, you name it. I suggest it is better to just believe these to be true. If you really want to, the proofs for these I imagine are easy to find. A more interesting theorem is the following: 

> Theorem 2.3.4 For any \\( n,m,p\in \omega \\) we have \\( m^{n+p}=m^n\cdot m^p \\)

Proof. Fix \\( m,n\in \omega \\). We then form the set

\\[ T=\\{ p\in \omega \ \vert \ m^{n+p}=m^n\cdot m^p \\}. \\]

Obviously if \\( T=\omega \\), then the theorem is true. We prove this by induction. The following shows that \\( 0\in T \\):

\\[ m^{n+0}=m^n=m^n\cdot 1=m^n\cdot m^0. \\]

Now suppose \\( k\in T \\), then

\\[ \begin{align\*} m^{n+k^+}&=m^{(n+k)^+} \newline &=m^{n+k}\cdot m \newline &=(m^n\cdot m^k)\cdot m \newline &=m^n\cdot (m^k\cdot m) \newline &=m^n\cdot m^{k^+} \end{align\*} \\]

Thus \\( k^+\in T. \quad \Box \\)

The proof method used here is similar to what would have been used were we to attempt the proofs of theorem 2.3.3. 
